theories/ml_lang/logrel/typing.v
@@ -168,5 +168,16 @@ Qed.
 Set Elimination Schemes.
 End IndDef.
 
+Fixpoint zip_types (an : list binder) (av : list type) : option (gmap string type) := match an, av with
+  nil, nil => Some ∅
+| (b::ar), (vx::vr) => option_map (binder_insert b vx) (zip_types ar vr)
+| _, _ => None end.
+
+Definition fun_typed (P : program_env) (Pt : program_type) (m : ml_function) : Prop := match m, Pt with
+  MlFun bs e, FunType ats rt => ∃ Γ', zip_types bs ats = Some Γ' ∧ typed P Γ' e rt end. 
+
+Definition program_typed (P : program_env) (p : ml_program) : Prop := 
+  map_Forall (λ s Pt, ∃ m, (p:gmap string _) !! s = Some m ∧ fun_typed P Pt m) (P : gmap string _).
+
 
 Notation "P ;; Γ ⊢ₜ e : τ" := (typed P Γ e τ) (at level 74, e, τ at next level).
