theories/examples/compression/buffers_proof_get.v
@@ -1,0 +1,61 @@
+From iris.proofmode Require Import coq_tactics reduction spec_patterns.
+From iris.proofmode Require Export tactics.
+From iris.prelude Require Import options.
+From melocoton Require Import named_props.
+From melocoton.interop Require Import basics basics_resources basics_constructions.
+From melocoton.interop Require Import lang weakestpre update_laws prims_proto.
+From melocoton.language Require Import weakestpre progenv.
+From melocoton.c_interop Require Import rules notation.
+From melocoton.ml_lang Require Import notation lang_instantiation.
+From melocoton.c_lang Require Import lang_instantiation.
+From melocoton.ml_lang Require primitive_laws proofmode.
+From melocoton.c_lang Require Import notation proofmode derived_laws.
+From melocoton.examples.compression Require Import buffers_specs buffers_laws buffers_code.
+
+Section Proofs.
+
+  Context `{SI:indexT}.
+  Context `{!heapG_C Σ, !heapG_ML Σ, !invG Σ, !primitive_laws.heapG_ML Σ, !wrapperG Σ}.
+
+
+  Lemma buf_get_correct Ψ :
+    prims_proto Ψ ||- buf_lib_prog :: wrap_proto (buf_get_spec_ML).
+  Proof.
+    iIntros (s ws Φ) "H". iNamed "H". iNamed "Hproto".
+    iSplit; first done.
+    iIntros (Φ'') "HΦ".
+    destruct lvs as [|lvb [|lvi [|??]]]; first done.
+    all: cbn; iDestruct "Hsim" as "(Hsimb&H)"; try done.
+    all: cbn; iDestruct "H" as "(->&H)"; try done.
+    destruct ws as [|wb [|wl [|??]]]; try (eapply Forall2_length in Hrepr; cbn in Hrepr; done).
+    eapply Forall2_cons_inv_l in Hrepr as (wγ&?&Hlγ&Hrepr&?); simplify_eq.
+    eapply Forall2_cons_inv_l in Hrepr as (wi&?&Hli&Hrepr&?); simplify_eq.
+    cbn. wp_call_direct.
+
+    iMod (bufToC with "HGC Hbuf Hsimb") as "(HGC&HBuf1&%&%&->)".
+    iNamed "HBuf1". iNamed "Hbuf".
+    iDestruct "HContent" as "(HContent&%Heqres)".
+    wp_apply (wp_readfield with "[$HGC $Hγbuf]"); [done..|].
+    iIntros (vγaux1 wγaux1) "(HGC&_&%Heq1&%Hreprγaux1)". cbv in Heq1; simplify_eq.
+    wp_apply (wp_readfield with "[$HGC $Hγaux]"); [done..|].
+    iIntros (vγfgn1 wγfgn1) "(HGC&_&%Heq1&%Hreprγfgn1)". cbv in Heq1; simplify_eq.
+    wp_apply (wp_read_foreign with "[$HGC $Hγfgnpto]"); [done..|].
+    iIntros "(HGC&Hγfgnpto)". wp_pure _.
+
+    wp_apply (wp_val2int with "HGC"); [done..|].
+    iIntros "HGC". wp_pure _.
+    wp_apply (wp_load_offset with "Hℓbuf").
+    { change (map ?a ?b) with (@fmap _ list_fmap _ _ a b). rewrite list_lookup_fmap Heqres.
+      cbn; done. }
+    iIntros "Hℓbuf".
+    iApply (wp_post_mono with "[HGC]").
+    1: wp_apply (wp_int2val with "HGC"); [done..|iIntros (w) "?"; iAccu].
+    iIntros (w) "(HGC&%Hww)".
+    iMod (bufToML_fixed with "HGC [Hγusedref HContent Hγfgnpto Hℓbuf] Hsimb") as "(HGC&HBuffer)"; last first.
+    { iModIntro. iApply "HΦ".
+      iApply ("Cont" with "HGC (HCont HBuffer) [//] [//]"). }
+    { do 6 iExists _. iSplit; first done. iFrameNamed.
+      do 1 iExists _. iFrameNamed. done. }
+  Qed.
+
+End Proofs.
